report positions of typedef
git-svn-id: https://projects.brucker.ch/hol-testgen/svn/HOL-TestGen/trunk/hol-testgen@13679 3260e6d1-4efc-4170-b0a7-36055960796d

C11-FrontEnd/C11-Interface.thy
@@ -196,11 +196,18 @@ end
 \<close>
 
 ML\<open>
-fun hook make_string f (_, (value, pos1, pos2)) thy =
+fun hook make_string f (_, (value, pos1, pos2)) _ thy =
   let
     val () = writeln (make_string value)
     val () = Position.reports_text [((Position.range (pos1, pos2) 
                                     |> Position.range_position, Markup.intensify), "")]
+  in f thy end
+
+fun hook' _ f (_, (_, pos1, pos2)) env thy =
+  let
+    val () = Position.reports_text [((Position.range (pos1, pos2) 
+                                    |> Position.range_position, Markup.intensify), "")]
+    val () = writeln ("ENV " ^ C_Env.string_of env)
   in f thy end
 
 fun setup s make_string (stack, env) thy =
@@ -211,10 +218,9 @@ fun setup s make_string (stack, env) thy =
           |> #2
           |> map_index I
           |> app (fn (i, (value, pos1, pos2)) => writeln ("   " ^ Int.toString (length stack - i) ^ " " ^ make_string value ^ " " ^ Position.here pos1 ^ " " ^ Position.here pos2))
-    val () = writeln ("ENV " ^ C_Env.string_of env)
   in thy end
 
-fun env s _ (stack, env) thy =
+fun setup' s _ (stack, env) thy =
   let
     val () = warning ("SHIFT  " ^ (case s of NONE => "" | SOME s => "\"" ^ s ^ "\" ") ^ Int.toString (length stack - 1) ^ "    +1 ")
     val () = writeln ("ENV " ^ C_Env.string_of env)
@@ -223,9 +229,11 @@ fun env s _ (stack, env) thy =
 
 setup \<open>ML_Antiquotation.inline @{binding hook}
                                (Args.context >> K ("hook " ^ ML_Pretty.make_string_fn ^ " I"))\<close>
+setup \<open>ML_Antiquotation.inline @{binding hook'}
+                               (Args.context >> K ("hook' " ^ ML_Pretty.make_string_fn ^ " I"))\<close>
 setup \<open>ML_Antiquotation.inline @{binding setup}
                                (Scan.peek (fn _ => Scan.option Args.text) >> (fn name => ("setup " ^ (case name of NONE => "NONE" | SOME s => "(SOME \"" ^ s ^ "\")") ^ " " ^ ML_Pretty.make_string_fn)))\<close>
-setup \<open>ML_Antiquotation.inline @{binding env}
-                               (Scan.peek (fn _ => Scan.option Args.text) >> (fn name => ("env " ^ (case name of NONE => "NONE" | SOME s => "(SOME \"" ^ s ^ "\")") ^ " " ^ ML_Pretty.make_string_fn)))\<close>
+setup \<open>ML_Antiquotation.inline @{binding setup'}
+                               (Scan.peek (fn _ => Scan.option Args.text) >> (fn name => ("setup' " ^ (case name of NONE => "NONE" | SOME s => "(SOME \"" ^ s ^ "\")") ^ " " ^ ML_Pretty.make_string_fn)))\<close>
 
 end
